theories/Interp/Sched.v
@@ -3,7 +3,8 @@ From ExtLib Require Import
      Structures.Monad.
 
 From CTree Require Import
-     Eq.
+     Eq
+     Interp.State.
 
 Import ITree.Basics.Basics.Monads.
 Import MonadNotation.
@@ -15,13 +16,15 @@ Open Scope monad_scope.
 
 Definition schedule {E M : Type -> Type}
 					 {FM : Functor M} {MM : Monad M} {IM : MonadIter M} {FoM : MonadTrigger E M}
-					 (h : forall n, M (fin n)) :
+           {CM : MonadChoice M}
+           (h : bool -> forall n, M (fin n)) :
 	ctree E ~> M :=
   fun R =>
 		iter (fun t =>
 				    match observe t with
 				    | RetF r => ret (inr r)
-				    | @ChoiceF _ _ _ _ n k => bind (h n) (fun x => ret (inl (k x)))
+				    | @ChoiceF _ _ _ b n k =>
+                bind (h b n) (fun x => ret (inl (k x)))
 				    | VisF e k => bind (mtrigger _ e) (fun x => ret (inl (k x)))
 				    end).
 
@@ -43,22 +46,129 @@ Definition pure {E R} := gfp (@fpure E R).
 (* Definition schedule_pure {E} (hV hI : forall n, fin n) : ctree E ~> ctree E := *)
 (*   schedule (fun n => Ret (h n)). *)
 
+#[global] Instance schedule_equ {E X} h :
+  Proper (@equ E X X eq ==> equ eq) (schedule h X).
+Proof.
+  cbn.
+  coinduction R CH.
+  intros. setoid_rewrite unfold_iter.
+  step in H. inv H.
+  - setoid_rewrite bind_ret_l. reflexivity.
+  - setoid_rewrite bind_bind. setoid_rewrite bind_trigger.
+    constructor. intros.
+    setoid_rewrite bind_ret_l.
+    step. constructor. intros _.
+    apply CH. apply REL.
+  - setoid_rewrite bind_bind.
+    upto_bind_eq.
+    setoid_rewrite bind_ret_l.
+    constructor. intros _.
+    apply CH. apply REL.
+Qed.
 
-Definition schedule_cst {E} (h : forall n, fin n) : ctree E ~> ctree E :=
-  schedule (fun n => Ret (h n)).
+Definition schedule_cst {E} (h : bool -> forall n, fin (S n)) : ctree E ~> ctree E :=
+  schedule (fun b n =>
+    match n with
+    | O => CTree.stuck b
+    | S n => Choice b 1 (fun _ => Ret (h b n))
+    end).
 
 Definition round_robin {E} : ctree E ~> stateT nat (ctree E).
+Proof.
   refine (schedule
-            (fun n m =>
+            (fun b n m =>
                (* m: branch to be scheduled
                   n: arity of the new node
                 *)
                match n as n' return (ctree E (nat * fin n')) with
-               | O => CTree.stuckI
-               | 1 => Ret (m, Fin.F1)
-               | S (S n) => (Ret (S m, @Fin.of_nat_lt (Nat.modulo m (S (S n))) _ _))
+               | O => CTree.stuck b
+               | S n => (Ret (S m, @Fin.of_nat_lt (Nat.modulo m (S n)) _ _))
                end
          )).
   apply (NPeano.Nat.mod_upper_bound).
   auto with arith.
 Defined.
+
+Theorem schedule_cst_refinement :
+  forall {E X} (h : bool -> forall n, fin (S n)) (t : ctree E X),
+  schedule_cst h _ t ≲ t.
+Proof.
+  intros until h. coinduction R CH. repeat intro.
+  do 3 red in H. remember (observe _) as os. genobs t' ot'.
+  assert (EQ : go os ≅ schedule_cst h X t \/ go os ≅ TauI (schedule_cst h X t)).
+  { left. rewrite Heqos. now rewrite <- ctree_eta. } clear Heqos.
+  apply (f_equal go) in Heqot'. eq2equ Heqot'.
+  rewrite <- ctree_eta in EQ0.
+  assert (exists u' : Trans.SS, trans l t u' /\ sst R t' u').
+  2: { destruct H0; exists x; destruct H0; assumption. }
+  setoid_rewrite <- EQ0. clear t' EQ0.
+  revert t EQ.
+  induction H; intros; subst.
+  - destruct EQ as [EQ|EQ]; symmetry in EQ.
+    setoid_rewrite unfold_iter in EQ.
+    setoid_rewrite (ctree_eta t0).
+    genobs t0 ot0. clear t0 Heqot0.
+    destruct ot0 eqn:?; subst.
+    + step in EQ. inv EQ.
+    + step in EQ. inv EQ.
+    + setoid_rewrite bind_bind in EQ.
+      setoid_rewrite bind_ret_l in EQ.
+      change t with (observe (go t)) in H.
+      rewrite trans__trans in H.
+      destruct n0.
+      * setoid_rewrite bind_choice in EQ.
+        apply equ_choice_invT in EQ as ?. destruct H0 as [<- _].
+        now eapply Fin.case0.
+      * setoid_rewrite bind_choice in EQ.
+        apply equ_choice_invT in EQ as ?. destruct H0 as [<- _].
+        destruct vis. { step in EQ. inv EQ. }
+        simple eapply equ_choice_invE with (x := x) in EQ.
+        rewrite bind_ret_l in EQ.
+        lapply (IHtrans_ (k0 (h false n0))).
+        -- intro. destruct H0 as (? & ? & ?).
+           etrans.
+        -- right. rewrite <- ctree_eta. now rewrite <- EQ.
+    + apply IHtrans_. left.
+      apply equ_choice_invT in EQ as ?. destruct H0 as [<- _]. rewrite <- ctree_eta.
+      simple apply equ_choice_invE with (x := x) in EQ. now rewrite EQ.
+  - destruct EQ. 2: { step in H0. inv H0. }
+    setoid_rewrite unfold_iter in H0. cbn in H0.
+    destruct (observe t0) eqn:?;
+      (try setoid_rewrite bind_choice in H0);
+      (try setoid_rewrite bind_trigger in H0);
+      (try destruct vis);
+      subst; try now step in H0; inv H0.
+    rewrite bind_bind in H0.
+    destruct n0.
+    + setoid_rewrite bind_choice in H0.
+      apply equ_choice_invT in H0 as ?. destruct H1 as [-> _].
+      now eapply Fin.case0.
+    + rewrite bind_choice in H0.
+      do 2 setoid_rewrite bind_ret_l in H0.
+      apply equ_choice_invT in H0 as ?. destruct H1 as [-> _].
+      simple apply equ_choice_invE with (x := x) in H0.
+      exists (k0 (h true n0)).
+      rewrite ctree_eta, Heqc. split; etrans.
+      rewrite <- H, H0, <- ctree_eta, sb_tauI.
+      apply CH.
+    + destruct n0; step in H0; inv H0.
+  - destruct EQ. 2: { step in H0. inv H0. }
+    setoid_rewrite unfold_iter in H0. cbn in H0.
+    destruct (observe t0) eqn:?;
+      try ((try destruct n); now step in H0; inv H0).
+    setoid_rewrite bind_trigger in H0. setoid_rewrite bind_vis in H0.
+    apply equ_vis_invT in H0 as ?. destruct H1.
+    apply equ_vis_invE in H0 as [-> ?].
+    setoid_rewrite bind_ret_l in H0.
+    exists (k0 x). eexists.
+    { rewrite ctree_eta, Heqc. etrans. }
+    rewrite <- H, H0, <- ctree_eta, sb_tauI. apply CH.
+  - destruct EQ. 2: { step in H. inv H. }
+    exists CTree.stuckI.
+    setoid_rewrite unfold_iter in H.
+    destruct (observe t) eqn:?;
+      try ((try destruct n); now step in H; inv H).
+    setoid_rewrite bind_ret_l in H.
+    + step in H. inv H. rewrite ctree_eta, Heqc.
+      split; etrans. rewrite choice0_always_stuck. reflexivity.
+Qed.
